feat(proj1): second exercise first task

proj1/src/Ex2.dfy
@@ -1,15 +1,26 @@
+function noRepsF(v: seq<nat>): bool
+{
+  forall i, j :: 0 <= i < |v| && 0 <= j < |v| ==> i != j ==> v[i] != v[j]
+}
+
 method noRepetitionsQuadratic(arr : array<nat>) returns (b: bool) 
+  ensures b == noRepsF(arr[..])
  {
   var i := 0; 
   b := true; 
 
   while (i < arr.Length) 
+      invariant 0 <= i <= arr.Length
+      invariant forall j, k :: 0 <= k < i && 0 <= j < arr.Length ==>
+                                    j != k ==> arr[j] != arr[k]
   {
 
     var v := arr[i];   
     var j := 0;
   
     while (j < arr.Length) 
+      invariant 0 <= j <= arr.Length
+      invariant forall k :: 0 <= k < j && k != i ==> arr[i] != arr[k]
     {
       var u := arr[j]; 
       if ((j != i) && (u == v)) {
@@ -20,12 +31,11 @@ method noRepetitionsQuadratic(arr : array<nat>) returns (b: bool)
     }
     i := i+1; 
   }
+
+  assert forall j, k :: 0 <= k < arr.Length && 0 <= j < arr.Length ==> j != k ==> arr[j] != arr[k];
 }
-
-
-
 
 method noRepetitionsLinear(arr : array<nat>) returns (b: bool) 
 {
-
+  // What ? I can't come up with a linear time array
 }
